src/lowparse/steel_st_array/LowParse.SteelST.ArrayPtr.fsti
@@ -154,3 +154,70 @@ val upd (#a:Type) (#value: v a) (r: t a) (i:SZ.size_t) (x:a)
                array_of value' == array_of value /\
                contents_of' value' == Seq.upd (contents_of' value) (SZ.size_v i) x
              )
+
+val set_array_perm
+  (#t: Type)
+  (a: array t)
+  (p: perm)
+: Ghost (array t)
+    (requires True)
+    (ensures (fun y -> len y == len a /\ array_perm y == p))
+
+val set_array_perm_idem
+  (#t: Type)
+  (a: array t)
+  (p1 p2: perm)
+: Lemma
+  (set_array_perm (set_array_perm a p1) p2 == set_array_perm a p2)
+  [SMTPat (set_array_perm (set_array_perm a p1) p2)]
+
+val set_array_perm_eq
+  (#t: Type)
+  (a: array t)
+: Lemma
+  (set_array_perm a (array_perm a) == a)
+  [SMTPat (set_array_perm a (array_perm a))]
+
+val set_array_perm_adjacent
+  (#t: Type)
+  (a1 a2: array t)
+  (p: perm)
+: Lemma
+  (requires (adjacent a1 a2))
+  (ensures (
+    merge_into (set_array_perm a1 p) (set_array_perm a2 p) (set_array_perm (merge a1 a2) p)
+  ))
+  [SMTPat (adjacent (set_array_perm a1 p) (set_array_perm a2 p))]
+
+val share
+  (#opened: _)
+  (#elt: Type)
+  (#x: v elt)
+  (a: t elt)
+  (p1 p2: perm)
+: STGhost (Ghost.erased (v elt & v elt)) opened
+    (arrayptr a x)
+    (fun res -> arrayptr a (fst res) `star` arrayptr a (snd res))
+    (array_perm (array_of x) == p1 `Steel.FractionalPermission.sum_perm` p2)
+    (fun res ->
+      contents_of' (fst res) == contents_of x /\
+      contents_of' (snd res) == contents_of x /\
+      array_of (fst res) == set_array_perm (array_of x) p1 /\
+      array_of (snd res) == set_array_perm (array_of x) p2
+    )
+
+val gather
+  (#opened: _)
+  (#elt: Type)
+  (#x1 #x2: v elt)
+  (a: t elt)
+: STGhost (v elt) opened
+    (arrayptr a x1 `star` arrayptr a x2)
+    (fun res -> arrayptr a res)
+    (array_of x1 == set_array_perm (array_of x2) (array_perm (array_of x1)))
+    (fun res ->
+      contents_of' res == contents_of x1 /\
+      contents_of' res == contents_of x2 /\
+      array_of res == set_array_perm (array_of x1) (array_perm (array_of x1) `Steel.FractionalPermission.sum_perm` array_perm (array_of x2))
+    )
+
